Lean4Lean/Std/ToExpr.lean
@@ -29,8 +29,8 @@ instance [ToLevel.{u}] : ToExpr PUnit.{u+1} where
   toExpr _ := mkConst ``PUnit.unit [toLevel.{u+1}]
   toTypeExpr := mkConst ``PUnit [toLevel.{u+1}]
 
-deriving instance ToExpr for String.Pos
-deriving instance ToExpr for Substring
+deriving instance ToExpr for String.Pos.Raw
+deriving instance ToExpr for Substring.Raw
 deriving instance ToExpr for SourceInfo
 deriving instance ToExpr for Syntax.Preresolved
 deriving instance ToExpr for Syntax
