Lean4Lean/Stream.lean
@@ -1,5 +1,0 @@
-
-structure NatStream where i := 0 deriving Inhabited
-
-instance : ToStream NatStream NatStream := ⟨id⟩
-instance : Stream NatStream Nat := ⟨fun ⟨r⟩ => some (r, ⟨r + 1⟩)⟩
