Lean4Lean/Verify/TypeChecker/Reduce.lean
@@ -13,9 +13,9 @@ theorem rawNatLitExt?.WF {c : VContext} (H : rawNatLitExt? e = some n) (he : c.T
     c.venv.contains ``Nat ∧ e' = .natLit n := by
   have : c.TrExprS (.lit (.natVal n)) e' := by
     unfold rawNatLitExt? at H; split at H <;> rename_i h
-    · cases H; exact .lit (he.eqv h)
+    · cases H; have := he.eqv h; exact .lit (this.nat_of_natZero c.Ewf c.hasPrimitives) this
     · unfold Expr.rawNatLit? at H; split at H <;> cases H; exact he
-  have hn := this.lit_has_type c.Ewf c.hasPrimitives
+  have hn := this.lit_has_type
   exact ⟨hn, this.unique (by trivial) (TrExprS.natLit c.hasPrimitives hn n).1⟩
 
 def reduceBinNatOpG (guard : Nat → Nat → Prop) [DecidableRel guard]
